% Appendix B

\chapter{Adjustment of Poisson's equation to the normalized form.}\label{app:AppendixB}
\lhead{Appendix B. \emph{Adjustment of Poisson's equation to a normalized form}}

The Poisson equation has the form

\begin{equation}\label{eq:B.1}
  \frac{d^{2}\varphi}{dx^2} = - \frac{\rho(x)}{\epsilon}
\end{equation}

If we consider that in a semiconductor with substrate concentration
$N_b$ (assume donors) an inhomogeneous concentration profile is formed
$N(x)$ (assume acceptors), we can write for the charge density
relation

\begin{equation}\label{eq:B.2}
  \rho(x) = - q (n(x) - p(x) + N(x) -N_b)
\end{equation}

The terms $n(x)$ and $p(x)$, which represent free charge carriers, are
expressed by the normalized potentials $u$ and $u_f$

\begin{subequations}\label{eq:B.3}
  \begin{align}
    u(x) &= \frac{E_i(\infty) - E_i(x)}{kT} = \frac{q\varphi(x)}{kT} \label{eq:B.3a}\\[0.3cm]
    u_f &= \frac{E_i(\infty) - E_f}{kT} \label{eq:B.3b}
  \end{align}
\end{subequations}

and using the substrate concentration

\begin{subequations}\label{eq:B.4}
  \begin{align}
    n(x) &= N_b {e}^{u(x)}\label{eq:B.4a}\\[0.3cm]
    p(x) &= n_i {e}\frac{E_i(x) - E_f}{kT} = n_i {e}^{u_f-u(x)} = N_b {e}^{2u_f-u(x)}\label{eq:B.4b}\\[0.3cm]
    \intertext{when we used the relation for the concentration of electrons in the substrate}
    n(\infty) &= N_b = n_i {e}\frac{E_f-E_i(\infty)}{kT} = n_i {e}^{-u_f}\label{eq:B.4c}
  \end{align}
\end{subequations}

Then the charge density can be written in the form

\begin{equation}\label{eq:B.5}
  \rho(x) = -qN_b(e^{u(x)} - e^{2u_f-u(x)} + \alpha(x) - 1)
\end{equation}

where $\alpha(x) = \frac{N(x)}{N_b}$

Substituting the charge density~\ref{eq:B.5} and the
substitution~\ref{eq:B.3} into the equation~\ref{eq:B.1}, we get

\begin{equation}\label{eq:B.6}
  \frac{d^{2}u(x)}{dx^2} = \frac{q^2N_b}{kT\varepsilon}(e^{u(x)} - e^{2u_f-u(x)} + \alpha(x) - 1)
\end{equation}

We introduce the effective Debay length

\begin{equation}\label{eq:B.7}
  L_D = {\Bigg[\frac{kT\varepsilon}{q^{2}N_b}\Bigg]}^{\frac{1}{2}}
\end{equation}

to which distance $x$ we normalize

\begin{equation}\label{eq:B.8}
  \xi = \frac{x}{L_D}
\end{equation}

We can write the Poisson equation in the normalized form

\begin{equation}\label{eq:B.9}
  \frac{d^{2}u(\xi)}{d\xi^2} = e^{u(\xi)} - e^{2u_f-u(\xi)} + \alpha(\xi) - 1
\end{equation}
